instead of unfold1_cmd_goal, eapply lemma_corresponding_to_command
In an "env everywhere" setting, where program_logic_goal_for!
adds a (map.get fs fname = Some fimpl) hypothesis.
Surprise #1: There's no case in straightline that handles if-then-else
Surprise #2: unfold1_... tactics are not the only place that depend
on conversion: There also exists a letexists in SPI that turns a
(WP (cmd.cond e _ _) ...) into an (exists v, eval e v /\ ...), and
probably more elsewhere.

bedrock2/src/bedrock2/WeakestPrecondition.v
@@ -2,10 +2,15 @@ Require Import coqutil.Macros.subst coqutil.Macros.unique coqutil.Map.Interface 
 Require Import Coq.ZArith.BinIntDef coqutil.Word.Interface coqutil.Word.Bitwidth.
 Require Import coqutil.dlet bedrock2.Syntax bedrock2.Semantics.
 
+Require Import coqutil.Map.Interface.
+Require coqutil.Map.SortedListString.
+
+#[export] Instance env: map.map String.string (list String.string * list String.string * Syntax.cmd.cmd) := SortedListString.map _.
+#[export] Instance env_ok: map.ok env := SortedListString.ok _.
+
 Section WeakestPrecondition.
   Context {width: Z} {BW: Bitwidth width} {word: word.word width} {mem: map.map word Byte.byte}.
   Context {locals: map.map String.string word}.
-  Context {env: map.map String.string (list String.string * list String.string * cmd)}.
   Context {ext_spec: ExtSpec}.
   Implicit Types (t : trace) (m : mem) (l : locals).
 
@@ -104,25 +109,25 @@ Section WeakestPrecondition.
   Section WithFunctionEnv.
     Context (e: env).
 
-    Inductive cmd' (c : Syntax.cmd) (t : trace) (m : mem) (l : locals)
+    Inductive cmd (c : Syntax.cmd) (t : trace) (m : mem) (l : locals)
       (post : (trace -> mem -> locals -> Prop)) : Prop :=
-    | mk_cmd' (_ : forall mc, exec e c t m l mc (fun t' m' l' mc' => post t' m' l')).
+    | mk_cmd (_ : forall mc, exec e c t m l mc (fun t' m' l' mc' => post t' m' l')).
 
-    Lemma invert_cmd': forall c t m l post,
-        cmd' c t m l post ->
+    Lemma invert_cmd: forall c t m l post,
+        cmd c t m l post ->
         forall mc, exec e c t m l mc (fun t' m' l' mc' => post t' m' l').
     Proof. intros. inversion H. apply H0. Qed.
 
-    Definition func' '(innames, outnames, c) (t : trace) (m : mem) (args : list word)
+    Definition func '(innames, outnames, c) (t : trace) (m : mem) (args : list word)
       (post : trace -> mem -> list word -> Prop) :=
       exists l, map.of_list_zip innames args = Some l /\
-      cmd' c t m l (fun t m l =>
+      cmd c t m l (fun t m l =>
         list_map (get l) outnames (fun rets =>
         post t m rets)).
 
-    Definition call' (fname: String.string) :=
+    Definition call (fname: String.string) :=
       match map.get e fname with
-      | Some fimpl => func' fimpl
+      | Some fimpl => func fimpl
       | None => fun _ _ _ _ => False
       end.
 
@@ -133,7 +138,7 @@ Section WeakestPrecondition.
       | H: _ /\ _ |- _ => destruct H
       | H: exists x, _ |- _ => let n := fresh x in destruct H as [n H]
       | |- _ => progress unfold dlet, dexpr, store in *
-      | H: cmd' _ _ _ _ _ |- _ => pose proof (invert_cmd' _ _ _ _ _ H); clear H
+      | H: cmd _ _ _ _ _ |- _ => pose proof (invert_cmd _ _ _ _ _ H); clear H
       | |- _ => constructor
       | |- _ => assumption
       | H: forall _: MetricLogging.MetricLog, _ |- _ => apply H
@@ -146,20 +151,20 @@ Section WeakestPrecondition.
       end.
     Ltac tac := repeat step.
 
-    Lemma wp_skip: forall t m l post, post t m l -> cmd' cmd.skip t m l post.
+    Lemma wp_skip: forall t m l post, post t m l -> cmd cmd.skip t m l post.
     Proof. tac. Qed.
 
     Lemma wp_set: forall x ev t m l post,
         (exists v, dexpr m l ev v /\
         dlet! l := map.put l x v in
         post t m l) ->
-        cmd' (cmd.set x ev) t m l post.
+        cmd (cmd.set x ev) t m l post.
     Proof. tac. Qed.
 
     Lemma wp_unset: forall x t m l post,
         (dlet! l := map.remove l x in
          post t m l) ->
-        cmd' (cmd.unset x) t m l post.
+        cmd (cmd.unset x) t m l post.
     Proof. tac. Qed.
 
     Lemma wp_store: forall sz ea ev t m l post,
@@ -167,7 +172,7 @@ Section WeakestPrecondition.
         exists v, dexpr m l ev v /\
         store sz m a v (fun m =>
         post t m l)) ->
-       cmd' (cmd.store sz ea ev) t m l post.
+       cmd (cmd.store sz ea ev) t m l post.
     Proof. tac. Qed.
 
     Lemma wp_stackalloc: forall x n c t m l post,
@@ -175,18 +180,18 @@ Section WeakestPrecondition.
         forall a mStack mCombined,
           anybytes a n mStack -> map.split mCombined m mStack ->
           dlet! l := map.put l x a in
-          cmd' c t mCombined l (fun t' mCombined' l' =>
+          cmd c t mCombined l (fun t' mCombined' l' =>
           exists m' mStack',
           anybytes a n mStack' /\ map.split mCombined' m' mStack' /\
           post t' m' l')) ->
-          cmd' (cmd.stackalloc x n c) t m l post.
+          cmd (cmd.stackalloc x n c) t m l post.
     Proof. tac. specialize H0 with (1 := H1) (2 := H2). tac. Qed.
 
     Lemma wp_cond: forall br ct cf t m l post,
         (exists v, dexpr m l br v /\
-        (word.unsigned v <> 0%Z -> cmd' ct t m l post) /\
-        (word.unsigned v = 0%Z -> cmd' cf t m l post)) ->
-        cmd' (cmd.cond br ct cf) t m l post.
+        (word.unsigned v <> 0%Z -> cmd ct t m l post) /\
+        (word.unsigned v = 0%Z -> cmd cf t m l post)) ->
+        cmd (cmd.cond br ct cf) t m l post.
     Proof.
       tac. destr.destr (Z.eqb (word.unsigned v0) 0).
       - specialize H1 with (1 := E). tac.
@@ -194,8 +199,8 @@ Section WeakestPrecondition.
     Qed.
 
     Lemma wp_seq: forall c1 c2 t m l post,
-        cmd' c1 t m l (fun t m l => cmd' c2 t m l post) ->
-        cmd' (cmd.seq c1 c2) t m l post.
+        cmd c1 t m l (fun t m l => cmd c2 t m l post) ->
+        cmd (cmd.seq c1 c2) t m l post.
     Proof.
       tac. eapply exec.weaken.
       { econstructor. 1: eapply H0. tac. }
@@ -208,10 +213,10 @@ Section WeakestPrecondition.
         (exists v, inv v t m l) /\
         (forall v t m l, inv v t m l ->
           exists b, dexpr m l e b /\
-          (word.unsigned b <> 0%Z -> cmd' c t m l (fun t' m l =>
+          (word.unsigned b <> 0%Z -> cmd c t m l (fun t' m l =>
             exists v', inv v' t' m l /\ lt v' v)) /\
           (word.unsigned b = 0%Z -> post t m l))) ->
-       cmd' (cmd.while e c) t m l post.
+       cmd (cmd.while e c) t m l post.
     Proof.
       intros. destruct H as (measure & lt & inv & Hwf & HInit & Hbody).
       destruct HInit as (v0 & HInit).
@@ -227,19 +232,19 @@ Section WeakestPrecondition.
         cbv beta. intros * (v' & HInv & HLt). eauto.
     Qed.
 
-    Lemma wp_call{env_ok: map.ok env}: forall binds fname arges t m l post,
+    Lemma wp_call: forall binds fname arges t m l post,
        (exists args, dexprs m l arges args /\
-        call' fname t m args (fun t m rets =>
+        call fname t m args (fun t m rets =>
           exists l', map.putmany_of_list_zip binds rets l = Some l' /\
           post t m l')) ->
-       cmd' (cmd.call binds fname arges) t m l post.
+       cmd (cmd.call binds fname arges) t m l post.
     Proof.
       tac.
       unfold dexprs in *.
       eapply exprs_sound in H. destruct H as (argvs & mc' & HEv & ?). subst argvs.
-      unfold call' in *.
+      unfold call in *.
       Tactics.destruct_one_match_hyp. 2: contradiction.
-      unfold func' in *.
+      unfold func in *.
       destruct p as ((argnames & retnames) & fbody).
       destruct H0 as (l1 & Hl1 & Hbody).
       inversion Hbody. clear Hbody. rename H into Hbody.
@@ -254,105 +259,28 @@ Section WeakestPrecondition.
           exists l', map.putmany_of_list_zip binds rets l = Some l' /\
           forall m', map.split m' mKeep mReceive ->
           post (cons ((mGive, action, args), (mReceive, rets)) t) m' l')) ->
-       cmd' (cmd.interact binds action arges) t m l post.
+       cmd (cmd.interact binds action arges) t m l post.
     Proof.
       tac.
       eapply exprs_sound in H. destruct H as (argvs & mc' & HEv & ?). subst argvs.
       tac.
     Qed.
   End WithFunctionEnv.
-
-  Section WithFunctions.
-    Context (call : String.string -> trace -> mem -> list word -> (trace -> mem -> list word -> Prop) -> Prop).
-    Definition cmd_body (rec:_->_->_->_->_->Prop) (c : cmd) (t : trace) (m : mem) (l : locals)
-             (post : trace -> mem -> locals -> Prop) : Prop :=
-      (* give value of each pure expression when stating its subproof *)
-      match c with
-      | cmd.skip => post t m l
-      | cmd.set x ev =>
-        exists v, dexpr m l ev v /\
-        dlet! l := map.put l x v in
-        post t m l
-      | cmd.unset x =>
-        dlet! l := map.remove l x in
-        post t m l
-      | cmd.store sz ea ev =>
-        exists a, dexpr m l ea a /\
-        exists v, dexpr m l ev v /\
-        store sz m a v (fun m =>
-        post t m l)
-      | cmd.stackalloc x n c =>
-        Z.modulo n (bytes_per_word width) = 0 /\
-        forall a mStack mCombined,
-          anybytes a n mStack -> map.split mCombined m mStack ->
-          dlet! l := map.put l x a in
-          rec c t mCombined l (fun t' mCombined' l' =>
-          exists m' mStack',
-          anybytes a n mStack' /\ map.split mCombined' m' mStack' /\
-          post t' m' l')
-      | cmd.cond br ct cf =>
-        exists v, dexpr m l br v /\
-        (word.unsigned v <> 0%Z -> rec ct t m l post) /\
-        (word.unsigned v = 0%Z -> rec cf t m l post)
-      | cmd.seq c1 c2 =>
-        rec c1 t m l (fun t m l => rec c2 t m l post)
-      | cmd.while e c =>
-        exists measure (lt:measure->measure->Prop) (inv:measure->trace->mem->locals->Prop),
-        Coq.Init.Wf.well_founded lt /\
-        (exists v, inv v t m l) /\
-        (forall v t m l, inv v t m l ->
-          exists b, dexpr m l e b /\
-          (word.unsigned b <> 0%Z -> rec c t m l (fun t' m l =>
-            exists v', inv v' t' m l /\ lt v' v)) /\
-          (word.unsigned b = 0%Z -> post t m l))
-      | cmd.call binds fname arges =>
-        exists args, dexprs m l arges args /\
-        call fname t m args (fun t m rets =>
-          exists l', map.putmany_of_list_zip binds rets l = Some l' /\
-          post t m l')
-      | cmd.interact binds action arges =>
-        exists args, dexprs m l arges args /\
-        exists mKeep mGive, map.split m mKeep mGive /\
-        ext_spec t mGive action args (fun mReceive rets =>
-          exists l', map.putmany_of_list_zip binds rets l = Some l' /\
-          forall m', map.split m' mKeep mReceive ->
-          post (cons ((mGive, action, args), (mReceive, rets)) t) m' l')
-      end.
-    Fixpoint cmd c := cmd_body cmd c.
-  End WithFunctions.
-
-  Definition func call '(innames, outnames, c) (t : trace) (m : mem) (args : list word) (post : trace -> mem -> list word -> Prop) :=
-      exists l, map.of_list_zip innames args = Some l /\
-      cmd call c t m l (fun t m l =>
-        list_map (get l) outnames (fun rets =>
-        post t m rets)).
-
-  Definition call_body rec (functions : list (String.string * (list String.string * list String.string * cmd.cmd)))
-                (fname : String.string) (t : trace) (m : mem) (args : list word)
-                (post : trace -> mem -> list word -> Prop) : Prop :=
-    match functions with
-    | nil => False
-    | cons (f, decl) functions =>
-      if String.eqb f fname
-      then func (rec functions) decl t m args post
-      else rec functions fname t m args post
-    end.
-  Fixpoint call functions := call_body call functions.
-
-  Definition program funcs main t m l post : Prop := cmd (call funcs) main t m l post.
 End WeakestPrecondition.
 
-Ltac unfold1_cmd e :=
-  lazymatch e with
-    @cmd ?width ?BW ?word ?mem ?locals ?ext_spec ?CA ?c ?t ?m ?l ?post =>
-    let c := eval hnf in c in
-    constr:(@cmd_body width BW word mem locals ext_spec CA
-                      (@cmd width BW word mem locals ext_spec CA) c t m l post)
+Ltac apply_rule_for_command c :=
+  lazymatch c with
+  | cmd.skip => eapply wp_skip
+  | cmd.set ?x ?ev => eapply wp_set
+  | cmd.unset ?x => eapply wp_unset
+  | cmd.store ?sz ?ea ?ev => eapply wp_store
+  | cmd.stackalloc ?x ?n ?c => eapply wp_stackalloc
+  | cmd.cond ?br ?ct ?cf => eapply wp_cond
+  | cmd.seq ?c1 ?c2 => eapply wp_seq
+  | cmd.while ?e ?c => eapply wp_while
+  | cmd.call ?binds ?fname ?arges => eapply wp_call
+  | cmd.interact ?binds ?action ?arges => eapply wp_interact
   end.
-Ltac unfold1_cmd_goal :=
-  let G := lazymatch goal with |- ?G => G end in
-  let G := unfold1_cmd G in
-  change G.
 
 Ltac unfold1_expr e :=
   lazymatch e with
@@ -374,18 +302,6 @@ Ltac unfold1_list_map e :=
 Ltac unfold1_list_map_goal :=
   let G := lazymatch goal with |- ?G => G end in
   let G := unfold1_list_map G in
-  change G.
-
-Ltac unfold1_call e :=
-  lazymatch e with
-    @call ?width ?BW ?word ?mem ?locals ?ext_spec ?fs ?fname ?t ?m ?l ?post =>
-    let fs := eval hnf in fs in
-    constr:(@call_body width BW word mem locals ext_spec
-                       (@call width BW word mem locals ext_spec) fs fname t m l post)
-  end.
-Ltac unfold1_call_goal :=
-  let G := lazymatch goal with |- ?G => G end in
-  let G := unfold1_call G in
   change G.
 
 Import Coq.ZArith.ZArith.
