bedrock2/src/bedrock2/Loops.v
@@ -11,15 +11,12 @@ From bedrock2 Require Import WeakestPrecondition WeakestPreconditionProperties.
 Section Loops.
   Context {width: Z} {BW: Bitwidth width} {word: word.word width} {mem: map.map word Byte.byte}.
   Context {locals: map.map String.string word}.
-  Context {env: map.map String.string (list String.string * list String.string * Syntax.cmd)}.
   Context {ext_spec: ExtSpec}.
   Context {word_ok : word.ok word} {mem_ok : map.ok mem}.
   Context {locals_ok : map.ok locals}.
-  Context {env_ok : map.ok env}.
   Context {ext_spec_ok : Semantics.ext_spec.ok ext_spec}.
 
-  Context {functions : list (String.string * (list String.string * list String.string * Syntax.cmd))}.
-  Let call := WeakestPrecondition.call functions.
+  Context {fs : env}.
 
   Lemma tailrec_localsmap_1ghost
     {e c t} {m: mem} {l} {post : trace -> mem -> locals -> Prop}
@@ -32,15 +29,16 @@ Section Loops.
     (Hbody: forall v g t m l,
       P v g t m l ->
       exists br, expr m l e (eq br) /\
-      (word.unsigned br <> 0%Z -> cmd call c t m l
+      (word.unsigned br <> 0%Z -> cmd fs c t m l
         (fun t' m' l' => exists v' g',
           P v' g' t' m' l' /\
           lt v' v /\
           (forall t'' m'' l'', Q v' g' t'' m'' l'' -> Q v g t'' m'' l''))) /\
       (word.unsigned br = 0%Z -> Q v g t m l))
     (Hpost: forall t m l, Q v0 g0 t m l -> post t m l)
-    : cmd call (cmd.while e c) t m l post.
+    : cmd fs (cmd.while e c) t m l post.
   Proof.
+    eapply wp_while.
     eexists measure, lt, (fun v t m l =>
       exists g, P v g t m l /\ forall t'' m'' l'', Q v g t'' m'' l'' -> Q v0 g0 t'' m'' l'').
     split; [assumption|].
@@ -50,8 +48,7 @@ Section Loops.
     destruct Hbody as (br & ? & Hbody). exists br; split; [assumption|].
     destruct Hbody as (Htrue & Hfalse). split; intros Hbr;
       [pose proof(Htrue Hbr)as Hpc|pose proof(Hfalse Hbr)as Hpc]; clear Hbr Htrue Hfalse.
-    { eapply Proper_cmd; [reflexivity..| | |eapply Hpc].
-      { eapply Proper_call; firstorder idtac. }
+    { eapply Proper_cmd; [ |eapply Hpc].
       intros tj mj lj (vj& gj & HPj & Hlt & Qji); eauto 9. }
     { eauto. }
   Qed.
@@ -67,16 +64,17 @@ Section Loops.
     (Hbody: forall v g t m l,
       P v g t m l ->
       exists br, expr m l e (eq br) /\
-      (word.unsigned br <> 0%Z -> cmd call c t m l
+      (word.unsigned br <> 0%Z -> cmd fs c t m l
         (fun t' m' l' => exists v' g',
           P v' g' t' m' l' /\
           lt v' v /\
           (forall t'' m'' l'', Q v' g' t'' m'' l'' -> Q v g t'' m'' l''))) /\
-      (word.unsigned br = 0%Z -> cmd call rest t m l (Q v g)))
-    : cmd call (cmd.seq (cmd.while e c) rest) t m l (Q v0 g0).
+      (word.unsigned br = 0%Z -> cmd fs rest t m l (Q v g)))
+    : cmd fs (cmd.seq (cmd.while e c) rest) t m l (Q v0 g0).
   Proof.
+    eapply wp_seq.
     cbn. eapply tailrec_localsmap_1ghost with
-      (Q := fun v g t m l => cmd call rest t m l (Q v g)).
+      (Q := fun v g t m l => cmd fs rest t m l (Q v g)).
     1: eassumption.
     1: exact Hpre.
     2: intros *; exact id.
@@ -85,14 +83,12 @@ Section Loops.
     destruct Hbody as (br & ? & Hbody). exists br; split; [assumption|].
     destruct Hbody as (Htrue & Hfalse). split; intros Hbr;
       [pose proof(Htrue Hbr)as Hpc|pose proof(Hfalse Hbr)as Hpc]; clear Hbr Htrue Hfalse.
-    { eapply Proper_cmd; [reflexivity..| | |eapply Hpc].
-      { eapply Proper_call; firstorder idtac. }
+    { eapply Proper_cmd; [ |eapply Hpc].
       intros tj mj lj (vj& gj & HPj & Hlt & Qji). do 2 eexists.
       split. 1: eassumption. split. 1: assumption.
       intros.
-      eapply Proper_cmd; [reflexivity..| | | ].
-      3: eassumption.
-      { eapply Proper_call; firstorder idtac. }
+      eapply Proper_cmd.
+      2: eassumption.
       intros tk mk lk HH. eapply Qji. assumption. }
     eapply Hpc.
   Qed.
@@ -166,10 +162,11 @@ Section Loops.
       invariant v t m l ->
       exists br, expr m l e (eq br) /\
          (word.unsigned br <> 0 ->
-          cmd call c t m l (fun t m l => exists v', invariant v' t m l /\ lt v' v)) /\
+          cmd fs c t m l (fun t m l => exists v', invariant v' t m l /\ lt v' v)) /\
          (word.unsigned br = 0 -> post t m l))
-    : cmd call (cmd.while e c) t m l post.
+    : cmd fs (cmd.while e c) t m l post.
   Proof.
+    eapply wp_while.
     eexists measure, lt, invariant.
     split. 1: exact Hwf.
     split. 1: eauto.
@@ -190,13 +187,13 @@ Section Loops.
       let l := reconstruct variables localstuple in
       exists br, expr m l e (eq br) /\
          (word.unsigned br <> 0 ->
-          cmd call c t m l (fun t m l =>
+          cmd fs c t m l (fun t m l =>
             Markers.unique (Markers.left (tuple.existss (fun localstuple =>
               enforce variables localstuple l /\
               Markers.right (Markers.unique (exists v',
                 tuple.apply (invariant v' t m) localstuple /\ lt v' v))))))) /\
          (word.unsigned br = 0 -> post t m l)))
-    : cmd call (cmd.while e c) t m l post.
+    : cmd fs (cmd.while e c) t m l post.
   Proof.
     eapply (while_localsmap (fun v t m l =>
       exists localstuple, enforce variables localstuple l /\
@@ -210,7 +207,7 @@ Section Loops.
     destruct Hbody as (br & Cond & Again & Done).
     exists br. split; [exact Cond|]. split; [|exact Done].
     intro NE. specialize (Again NE).
-    eapply Proper_cmd; [eapply Proper_call| |eapply Again].
+    eapply Proper_cmd; [ |eapply Again].
     cbv [Morphisms.pointwise_relation Basics.impl Markers.right Markers.unique Markers.left] in *.
     intros t' m' l' Ex.
     eapply hlist.existss_exists in Ex. cbv beta in Ex. destruct Ex as (ls & E & v' & Inv' & LT).
@@ -234,7 +231,7 @@ Section Loops.
       match tuple.apply (hlist.apply (spec v) g t m) l with S_ =>
       S_.(1) ->
       Markers.unique (Markers.left (exists br, expr m localsmap e (eq br) /\ Markers.right (
-      (word.unsigned br <> 0%Z -> cmd call c t m localsmap
+      (word.unsigned br <> 0%Z -> cmd fs c t m localsmap
         (fun t' m' localsmap' =>
           Markers.unique (Markers.left (hlist.existss (fun l' => enforce variables l' localsmap' /\ Markers.right (
           Markers.unique (Markers.left (hlist.existss (fun g' => exists v',
@@ -244,9 +241,10 @@ Section Loops.
             forall T M, hlist.foralls (fun L => tuple.apply (S'.(2) T M) L -> tuple.apply (S_.(2) T M) L)) end))))))))) /\
       (word.unsigned br = 0%Z -> tuple.apply (S_.(2) t m) l))))end))))
     (Hpost : match (tuple.apply (hlist.apply (spec v0) g0 t m) l0).(2) with Q0 => forall t m, hlist.foralls (fun l =>  tuple.apply (Q0 t m) l -> post t m (reconstruct variables l))end)
-    , cmd call (cmd.while e c) t m localsmap post ).
+    , cmd fs (cmd.while e c) t m localsmap post ).
   Proof.
     eapply hlist_forall_foralls; intros g0 **.
+    eapply wp_while.
     eexists measure, lt, (fun vi ti mi localsmapi =>
       exists gi li, localsmapi = reconstruct variables li /\
       match tuple.apply (hlist.apply (spec vi) gi ti mi) li with S_ =>
@@ -259,8 +257,7 @@ Section Loops.
     destruct (hlist.foralls_forall (hlist.foralls_forall (Hbody vi) gi ti mi) _ ltac:(eassumption)) as (br&?&X).
     exists br; split; [assumption|]. destruct X as (Htrue&Hfalse). split; intros Hbr;
       [pose proof(Htrue Hbr)as Hpc|pose proof(Hfalse Hbr)as Hpc]; clear Hbr Htrue Hfalse.
-    { eapply Proper_cmd; [reflexivity..| | |eapply Hpc].
-      { eapply Proper_call; firstorder idtac. }
+    { eapply Proper_cmd; [ |eapply Hpc].
       intros tj mj lmapj Hlj; eapply hlist.existss_exists in Hlj.
       destruct Hlj as (lj&Elj&HE); eapply reconstruct_enforce in Elj; subst lmapj.
       eapply hlist.existss_exists in HE. destruct HE as (l&?&?&?&HR).
@@ -279,7 +276,7 @@ Section Loops.
       let S := spec v t m l in let (P, Q) := S in
       P ->
       exists br, expr m l e (eq br) /\
-      (word.unsigned br <> 0%Z -> cmd call c t m l
+      (word.unsigned br <> 0%Z -> cmd fs c t m l
         (fun t' m' l' => exists v',
           let S' := spec v' t' m' l' in let '(P', Q') := S' in
           P' /\
@@ -287,8 +284,9 @@ Section Loops.
           forall T M L, Q' T M L -> Q T M L)) /\
       (word.unsigned br = 0%Z -> Q t m l))
     (Hpost : forall t m l, Q0 t m l -> post t m l)
-    : cmd call (cmd.while e c) t m l post.
+    : cmd fs (cmd.while e c) t m l post.
   Proof.
+    eapply wp_while.
     eexists measure, lt, (fun v t m l =>
       let S := spec v t m l in let '(P, Q) := S in
       P /\ forall T M L, Q T M L -> Q0 T M L).
@@ -299,8 +297,7 @@ Section Loops.
     destruct (Hbody _ _ _ _ ltac:(eassumption)) as (br&?&X); exists br; split; [assumption|].
     destruct X as (Htrue&Hfalse). split; intros Hbr;
       [pose proof(Htrue Hbr)as Hpc|pose proof(Hfalse Hbr)as Hpc]; clear Hbr Htrue Hfalse.
-    { eapply Proper_cmd; [reflexivity..| | |eapply Hpc].
-      { eapply Proper_call; firstorder idtac. }
+    { eapply Proper_cmd; [ |eapply Hpc].
       intros tj mj lj (vj&dP&?&dQ); eauto 9. }
     { eauto. }
   Qed.
@@ -328,12 +325,13 @@ Section Loops.
     (Henter : exists br, expr m l e (eq br) /\ (word.unsigned br = 0%Z -> post t m l))
     (v0 : measure) (Hpre : invariant v0 t m l)
     (Hbody : forall v t m l, invariant v t m l ->
-       cmd call c t m l (fun t m l =>
+       cmd fs c t m l (fun t m l =>
          exists br, expr m l e (eq br) /\
          (word.unsigned br <> 0 -> exists v', invariant v' t m l /\ lt v' v) /\
          (word.unsigned br =  0 -> post t m l)))
-    : cmd call (cmd.while e c) t m l post.
+    : cmd fs (cmd.while e c) t m l post.
   Proof.
+    eapply wp_while.
     eexists (option measure), (with_bottom lt), (fun ov t m l =>
       exists br, expr m l e (eq br) /\
       ((word.unsigned br <> 0 -> exists v, ov = Some v /\ invariant v t m l) /\
@@ -349,7 +347,7 @@ Section Loops.
     intros vi ti mi li (br&Ebr&Hcontinue&Hexit).
     eexists; split; [eassumption|]; split.
     { intros Hc; destruct (Hcontinue Hc) as (v&?&Hinv); subst.
-      eapply Proper_cmd; [| |eapply Hbody; eassumption]; [eapply Proper_call|].
+      eapply Proper_cmd; [ |eapply Hbody; eassumption].
       intros t' m' l' (br'&Ebr'&Hinv'&Hpost').
       destruct (BinInt.Z.eq_dec (word.unsigned br') 0).
       { exists None; split; try constructor.
@@ -374,7 +372,7 @@ Section Loops.
       let S := spec v t m l in let (P, Q) := S in
       P ->
       exists br, expr m l e (eq br) /\
-      (word.unsigned br <> 0%Z -> cmd call c t m l
+      (word.unsigned br <> 0%Z -> cmd fs c t m l
         (fun t' m' l' =>
           (exists br, expr m' l' e (eq br) /\ word.unsigned br = 0 /\ Q t' m' l') \/
           exists v', let S' := spec v' t' m' l' in let '(P', Q') := S' in
@@ -383,8 +381,9 @@ Section Loops.
           forall T M L, Q' T M L -> Q T M L)) /\
       (word.unsigned br = 0%Z -> Q t m l))
     (Hpost : forall t m l, Q0 t m l -> post t m l)
-    : cmd call (cmd.while e c) t m l post.
+    : cmd fs (cmd.while e c) t m l post.
   Proof.
+    eapply wp_while.
     eexists (option measure), (with_bottom lt), (fun v t m l =>
       match v with
       | None => exists br, expr m l e (eq br) /\ word.unsigned br = 0 /\ Q0 t m l
@@ -399,8 +398,7 @@ Section Loops.
     { destruct (Hbody _ _ _ _ ltac:(eassumption)) as (br&?&X); exists br; split; [assumption|].
       destruct X as (Htrue&Hfalse). split; intros Hbr;
         [pose proof(Htrue Hbr)as Hpc|pose proof(Hfalse Hbr)as Hpc]; eauto.
-      eapply Proper_cmd; [reflexivity..| | |eapply Hpc].
-      { eapply Proper_call; firstorder idtac. }
+      eapply Proper_cmd; [ |eapply Hpc].
       intros tj mj lj [(br'&Hbr'&Hz&HQ)|(vj&dP&?&dQ)];
           [exists None | exists (Some vj)]; cbn [with_bottom]; eauto 9. }
     repeat esplit || eauto || intros; contradiction.
@@ -423,7 +421,7 @@ Section Loops.
       match tuple.apply (hlist.apply (spec v) g t m) l with S_ =>
       S_.(1) ->
       Markers.unique (Markers.left (exists br, expr m localsmap e (eq br) /\ Markers.right (
-      (word.unsigned br <> 0%Z -> cmd call c t m localsmap
+      (word.unsigned br <> 0%Z -> cmd fs c t m localsmap
         (fun t' m' localsmap' =>
           Markers.unique (Markers.left (hlist.existss (fun l' => enforce variables l' localsmap' /\ Markers.right (
           Markers.unique (Markers.left (exists br, expr m' localsmap' e (eq br) /\ Markers.right ( word.unsigned br = 0 /\ tuple.apply (S_.(2) t' m') l') ) ) \/
@@ -434,9 +432,10 @@ Section Loops.
             forall T M, hlist.foralls (fun L => tuple.apply (S'.(2) T M) L -> tuple.apply (S_.(2) T M) L)) end))))))))) /\
       (word.unsigned br = 0%Z -> tuple.apply (S_.(2) t m) l))))end))))
     (Hpost : match (tuple.apply (hlist.apply (spec v0) g0 t m) l0).(2) with Q0 => forall t m, hlist.foralls (fun l =>  tuple.apply (Q0 t m) l -> post t m (reconstruct variables l))end)
-    , cmd call (cmd.while e c) t m localsmap post ).
+    , cmd fs (cmd.while e c) t m localsmap post ).
   Proof.
     eapply hlist_forall_foralls; intros g0 **.
+    eapply wp_while.
     eexists (option measure), (with_bottom lt), (fun vi ti mi localsmapi =>
       exists li, localsmapi = reconstruct variables li /\
       match vi with None => exists br, expr mi localsmapi e (eq br) /\ word.unsigned br = 0 /\ tuple.apply ((tuple.apply (hlist.apply (spec v0) g0 t m) l0).(2) ti mi) li | Some vi =>
@@ -455,8 +454,7 @@ Section Loops.
     destruct (hlist.foralls_forall (hlist.foralls_forall (Hbody vi) gi ti mi) _ ltac:(eassumption)) as (br&?&X).
     exists br; split; [assumption|]. destruct X as (Htrue&Hfalse). split; intros Hbr;
       [pose proof(Htrue Hbr)as Hpc|pose proof(Hfalse Hbr)as Hpc]; clear Hbr Htrue Hfalse.
-    { eapply Proper_cmd; [reflexivity..| | |eapply Hpc].
-      { eapply Proper_call; firstorder idtac. }
+    { eapply Proper_cmd; [ |eapply Hpc].
       intros tj mj lmapj Hlj; eapply hlist.existss_exists in Hlj.
       destruct Hlj as (lj&Elj&HE); eapply reconstruct_enforce in Elj; subst lmapj.
       destruct HE as [(br'&Hevalr'&Hz'&Hdone)|HE].
@@ -480,11 +478,11 @@ Section Loops.
     (v0 : measure) (Hpre : tuple.apply (invariant v0 t m) localstuple)
     (Hbody : forall v t m, tuple.foralls (fun localstuple =>
       tuple.apply (invariant v t m) localstuple ->
-       cmd call c t m (reconstruct variables localstuple) (fun t m l =>
+       cmd fs c t m (reconstruct variables localstuple) (fun t m l =>
          exists br, expr m l e (eq br) /\
          (word.unsigned br <> 0 -> Markers.unique (Markers.left (tuple.existss (fun localstuple => enforce variables localstuple l /\ Markers.right (Markers.unique (exists v', tuple.apply (invariant v' t m) localstuple /\ lt v' v)))))) /\
          (word.unsigned br =  0 -> post t m l))))
-    : cmd call (cmd.while e c) t m l post.
+    : cmd fs (cmd.while e c) t m l post.
   Proof.
     eapply (atleastonce_localsmap (fun v t m l => exists localstuple, Logic.and (enforce variables localstuple l) (tuple.apply (invariant v t m) localstuple))); eauto.
     intros vi ti mi li (?&X&Y).
@@ -492,7 +490,7 @@ Section Loops.
     eapply hlist.foralls_forall in Hbody.
     specialize (Hbody Y).
     rewrite <-(reconstruct_enforce _ _ _ X) in Hbody.
-    eapply Proper_cmd; [eapply Proper_call| |eapply Hbody].
+    eapply Proper_cmd; [ |eapply Hbody].
     intros t' m' l' (?&?&HH&?).
     eexists; split; eauto.
     split; intros; eauto.
@@ -504,7 +502,7 @@ Section Loops.
   Lemma while_zero_iterations {e c t l} {m : mem} {post : _->_->_-> Prop}
     (HCond: expr m l e (eq (word.of_Z 0)))
     (HPost: post t m l)
-    : cmd call (cmd.while e c) t m l post.
+    : cmd fs (cmd.while e c) t m l post.
   Proof.
     eapply (while_localsmap (fun n t' m' l' => t' = t /\ m' = m /\ l' = l) (PeanoNat.Nat.lt_wf 0) 0%nat).
     1: unfold split; auto. intros *. intros (? & ? & ?). subst.
@@ -525,14 +523,15 @@ Section Loops.
     (Hpre : (P v0 t l * R0) m)
     (Hbody : forall v t m l R, (P v t l * R) m ->
       exists br, expr m l e (eq br) /\
-      (word.unsigned br <> 0%Z -> cmd call c t m l
+      (word.unsigned br <> 0%Z -> cmd fs c t m l
         (fun t' m' l' => exists v' dR, (P v' t' l' * (R * dR)) m' /\
           lt v' v /\
           forall T L, Q v' T L * dR ==> Q v T L)) /\
       (word.unsigned br = 0%Z -> (Q v t l * R) m))
     (Hpost : forall t m l, (Q v0 t l * R0) m -> post t m l)
-    : cmd call (cmd.while e c) t m l post.
+    : cmd fs (cmd.while e c) t m l post.
   Proof.
+    eapply wp_while.
     eexists measure, lt, (fun v t m l => exists R, (P v t l * R) m /\
                           forall T L, Q v T L * R ==> Q v0 T L * R0).
     split; [assumption|].
@@ -541,8 +540,7 @@ Section Loops.
     destruct (Hbody _ _ _ _ _ ltac:(eassumption)) as (br&?&X); exists br; split; [assumption|].
     destruct X as (Htrue&Hfalse). split; intros Hbr;
       [pose proof(Htrue Hbr)as Hpc|pose proof(Hfalse Hbr)as Hpc]; clear Hbr Htrue Hfalse.
-    { eapply Proper_cmd; [reflexivity..| | |eapply Hpc].
-      { eapply Proper_call; firstorder idtac. }
+    { eapply Proper_cmd; [ |eapply Hpc].
       intros tj mj lj (vj&dR&dP&?&dQ).
       exists vj; split; [|assumption].
       exists (Ri * dR); split; [assumption|].
